Risc0/Gadgets/OneHot20/Constraints/WeakestPresPart14.lean
@@ -10,32 +10,42 @@ open MLIRNotation
 -- The state obtained by running Code.part14 on st
 def part14_state (st: State) : State :=
   
-        ((((st[felts][{ name := "%62" }] ←
-                Option.get! (State.felts st { name := "%61" }) *
-                  Option.get! (State.felts st { name := "%14" }))[felts][{ name := "%63" }] ←
-              Option.get! (State.felts st { name := "%60" }) +
-                Option.get! (State.felts st { name := "%61" }) *
-                  Option.get! (State.felts st { name := "%14" }))[felts][{ name := "%15" }] ←
-            16)["%64"] ←ₛ
-          getImpl st { name := "data" } 0 16) 
+        ((((st[felts][{ name := "%57" }] ←
+                Option.get! (State.felts st { name := "%8" }) -
+                  Option.get! (State.felts st { name := "%56" }))[props][{ name := "%58" }] ←
+              (Option.get! (State.props st { name := "%43" }) ∧
+                Option.get! (State.felts st { name := "%8" }) - Option.get! (State.felts st { name := "%56" }) =
+                  0))["%60"] ←ₛ
+            getImpl st { name := "data" } 0 16)[felts][{ name := "%61" }] ←
+          Option.get!
+              (State.felts
+                (((st[felts][{ name := "%57" }] ←
+                      Option.get! (State.felts st { name := "%8" }) -
+                        Option.get! (State.felts st { name := "%56" }))[props][{ name := "%58" }] ←
+                    (Option.get! (State.props st { name := "%43" }) ∧
+                      Option.get! (State.felts st { name := "%8" }) - Option.get! (State.felts st { name := "%56" }) =
+                        0))["%60"] ←ₛ
+                  getImpl st { name := "data" } 0 16)
+                { name := "%60" }) *
+            Option.get! (State.felts st { name := "%0" })) 
 
 def part14_drops (st: State) : State :=
-  State.dropFelts (State.dropFelts (State.dropFelts (st) ⟨"%60"⟩) ⟨"%14"⟩) ⟨"%62"⟩
+  State.dropFelts (State.dropFelts (State.dropFelts (State.dropFelts (State.dropFelts (st) ⟨"%0"⟩) ⟨"%56"⟩) ⟨"%8"⟩) ⟨"%57"⟩) ⟨"%60"⟩
 
 -- Run the program from part14 onwards by using part14_state rather than Code.part14
 def part14_state_update (st: State): State :=
-  Γ (part14_drops (part14_state st)) ⟦Code.part15;dropfelt ⟨"%63"⟩;dropfelt ⟨"%15"⟩;dropfelt ⟨"%65"⟩;Code.part16;dropfelt ⟨"%66"⟩;dropfelt ⟨"%16"⟩;dropfelt ⟨"%68"⟩;Code.part17;dropfelt ⟨"%69"⟩;dropfelt ⟨"%17"⟩;dropfelt ⟨"%71"⟩;Code.part18;dropfelt ⟨"%72"⟩;dropfelt ⟨"%18"⟩;dropfelt ⟨"%74"⟩;dropfelt ⟨"%75"⟩;dropfelt ⟨"%20"⟩;Code.part19;dropfelt ⟨"%76"⟩;Code.part20;dropfelt ⟨"%79"⟩;dropfelt ⟨"%80"⟩;dropfelt ⟨"%82"⟩;Code.part21;dropfelt ⟨"%21"⟩;dropfelt ⟨"%78"⟩;dropfelt ⟨"%83"⟩;dropfelt ⟨"%86"⟩;Code.part22;dropfelt ⟨"%22"⟩;dropfelt ⟨"%85"⟩;dropfelt ⟨"%87"⟩;dropfelt ⟨"%90"⟩;Code.part23;dropfelt ⟨"%25"⟩;dropfelt ⟨"%89"⟩;dropfelt ⟨"%91"⟩;dropfelt ⟨"%94"⟩;Code.part24;dropfelt ⟨"%28"⟩;dropfelt ⟨"%93"⟩;dropfelt ⟨"%95"⟩;dropfelt ⟨"%98"⟩;Code.part25;dropfelt ⟨"%31"⟩;dropfelt ⟨"%97"⟩;dropfelt ⟨"%99"⟩;dropfelt ⟨"%102"⟩;Code.part26;dropfelt ⟨"%34"⟩;dropfelt ⟨"%101"⟩;dropfelt ⟨"%103"⟩;dropfelt ⟨"%106"⟩;Code.part27;dropfelt ⟨"%37"⟩;dropfelt ⟨"%105"⟩;dropfelt ⟨"%107"⟩;dropfelt ⟨"%110"⟩;Code.part28;dropfelt ⟨"%40"⟩;dropfelt ⟨"%109"⟩;dropfelt ⟨"%111"⟩;dropfelt ⟨"%114"⟩;Code.part29;dropfelt ⟨"%43"⟩;dropfelt ⟨"%113"⟩;dropfelt ⟨"%115"⟩;dropfelt ⟨"%118"⟩;Code.part30;dropfelt ⟨"%46"⟩;dropfelt ⟨"%117"⟩;dropfelt ⟨"%119"⟩;dropfelt ⟨"%122"⟩;Code.part31;dropfelt ⟨"%49"⟩;dropfelt ⟨"%121"⟩;dropfelt ⟨"%123"⟩;dropfelt ⟨"%126"⟩;Code.part32;dropfelt ⟨"%52"⟩;dropfelt ⟨"%125"⟩;dropfelt ⟨"%127"⟩;dropfelt ⟨"%130"⟩;Code.part33;dropfelt ⟨"%55"⟩;dropfelt ⟨"%129"⟩;dropfelt ⟨"%131"⟩;dropfelt ⟨"%134"⟩;Code.part34;dropfelt ⟨"%58"⟩;dropfelt ⟨"%133"⟩;dropfelt ⟨"%135"⟩;dropfelt ⟨"%138"⟩;Code.part35;dropfelt ⟨"%61"⟩;dropfelt ⟨"%137"⟩;dropfelt ⟨"%139"⟩;dropfelt ⟨"%142"⟩;Code.part36;dropfelt ⟨"%64"⟩;dropfelt ⟨"%141"⟩;dropfelt ⟨"%143"⟩;dropfelt ⟨"%146"⟩;Code.part37;dropfelt ⟨"%67"⟩;dropfelt ⟨"%145"⟩;dropfelt ⟨"%147"⟩;dropfelt ⟨"%150"⟩;Code.part38;dropfelt ⟨"%70"⟩;dropfelt ⟨"%149"⟩;dropfelt ⟨"%151"⟩;dropfelt ⟨"%154"⟩;Code.part39;dropfelt ⟨"%19"⟩;dropfelt ⟨"%73"⟩;dropfelt ⟨"%77"⟩;dropfelt ⟨"%0"⟩;dropfelt ⟨"%81"⟩;dropfelt ⟨"%84"⟩;dropfelt ⟨"%88"⟩;dropfelt ⟨"%92"⟩;dropfelt ⟨"%96"⟩;dropfelt ⟨"%100"⟩;dropfelt ⟨"%104"⟩;dropfelt ⟨"%108"⟩;dropfelt ⟨"%112"⟩;dropfelt ⟨"%116"⟩;dropfelt ⟨"%120"⟩;dropfelt ⟨"%124"⟩;dropfelt ⟨"%128"⟩;dropfelt ⟨"%132"⟩;dropfelt ⟨"%136"⟩;dropfelt ⟨"%140"⟩;dropfelt ⟨"%144"⟩;dropfelt ⟨"%148"⟩;dropfelt ⟨"%152"⟩;dropfelt ⟨"%153"⟩;dropfelt ⟨"%155"⟩;dropfelt ⟨"%156"⟩;dropfelt ⟨"%157"⟩;dropfelt ⟨"%158"⟩;dropfelt ⟨"%159"⟩⟧
+  Γ (part14_drops (part14_state st)) ⟦Code.part15;dropfelt ⟨"%61"⟩;dropfelt ⟨"%59"⟩;dropfelt ⟨"%62"⟩;dropfelt ⟨"%7"⟩;Code.part16;dropfelt ⟨"%6"⟩;dropfelt ⟨"%28"⟩;dropfelt ⟨"%43"⟩;dropfelt ⟨"%58"⟩;dropfelt ⟨"%63"⟩;dropfelt ⟨"%64"⟩⟧
 
 -- Prove that substituting part14_state for Code.part14 produces the same result
 lemma part14_wp {st : State} :
-  Code.getReturn (MLIR.runProgram (Code.part14;dropfelt ⟨"%60"⟩;dropfelt ⟨"%14"⟩;dropfelt ⟨"%62"⟩;Code.part15;dropfelt ⟨"%63"⟩;dropfelt ⟨"%15"⟩;dropfelt ⟨"%65"⟩;Code.part16;dropfelt ⟨"%66"⟩;dropfelt ⟨"%16"⟩;dropfelt ⟨"%68"⟩;Code.part17;dropfelt ⟨"%69"⟩;dropfelt ⟨"%17"⟩;dropfelt ⟨"%71"⟩;Code.part18;dropfelt ⟨"%72"⟩;dropfelt ⟨"%18"⟩;dropfelt ⟨"%74"⟩;dropfelt ⟨"%75"⟩;dropfelt ⟨"%20"⟩;Code.part19;dropfelt ⟨"%76"⟩;Code.part20;dropfelt ⟨"%79"⟩;dropfelt ⟨"%80"⟩;dropfelt ⟨"%82"⟩;Code.part21;dropfelt ⟨"%21"⟩;dropfelt ⟨"%78"⟩;dropfelt ⟨"%83"⟩;dropfelt ⟨"%86"⟩;Code.part22;dropfelt ⟨"%22"⟩;dropfelt ⟨"%85"⟩;dropfelt ⟨"%87"⟩;dropfelt ⟨"%90"⟩;Code.part23;dropfelt ⟨"%25"⟩;dropfelt ⟨"%89"⟩;dropfelt ⟨"%91"⟩;dropfelt ⟨"%94"⟩;Code.part24;dropfelt ⟨"%28"⟩;dropfelt ⟨"%93"⟩;dropfelt ⟨"%95"⟩;dropfelt ⟨"%98"⟩;Code.part25;dropfelt ⟨"%31"⟩;dropfelt ⟨"%97"⟩;dropfelt ⟨"%99"⟩;dropfelt ⟨"%102"⟩;Code.part26;dropfelt ⟨"%34"⟩;dropfelt ⟨"%101"⟩;dropfelt ⟨"%103"⟩;dropfelt ⟨"%106"⟩;Code.part27;dropfelt ⟨"%37"⟩;dropfelt ⟨"%105"⟩;dropfelt ⟨"%107"⟩;dropfelt ⟨"%110"⟩;Code.part28;dropfelt ⟨"%40"⟩;dropfelt ⟨"%109"⟩;dropfelt ⟨"%111"⟩;dropfelt ⟨"%114"⟩;Code.part29;dropfelt ⟨"%43"⟩;dropfelt ⟨"%113"⟩;dropfelt ⟨"%115"⟩;dropfelt ⟨"%118"⟩;Code.part30;dropfelt ⟨"%46"⟩;dropfelt ⟨"%117"⟩;dropfelt ⟨"%119"⟩;dropfelt ⟨"%122"⟩;Code.part31;dropfelt ⟨"%49"⟩;dropfelt ⟨"%121"⟩;dropfelt ⟨"%123"⟩;dropfelt ⟨"%126"⟩;Code.part32;dropfelt ⟨"%52"⟩;dropfelt ⟨"%125"⟩;dropfelt ⟨"%127"⟩;dropfelt ⟨"%130"⟩;Code.part33;dropfelt ⟨"%55"⟩;dropfelt ⟨"%129"⟩;dropfelt ⟨"%131"⟩;dropfelt ⟨"%134"⟩;Code.part34;dropfelt ⟨"%58"⟩;dropfelt ⟨"%133"⟩;dropfelt ⟨"%135"⟩;dropfelt ⟨"%138"⟩;Code.part35;dropfelt ⟨"%61"⟩;dropfelt ⟨"%137"⟩;dropfelt ⟨"%139"⟩;dropfelt ⟨"%142"⟩;Code.part36;dropfelt ⟨"%64"⟩;dropfelt ⟨"%141"⟩;dropfelt ⟨"%143"⟩;dropfelt ⟨"%146"⟩;Code.part37;dropfelt ⟨"%67"⟩;dropfelt ⟨"%145"⟩;dropfelt ⟨"%147"⟩;dropfelt ⟨"%150"⟩;Code.part38;dropfelt ⟨"%70"⟩;dropfelt ⟨"%149"⟩;dropfelt ⟨"%151"⟩;dropfelt ⟨"%154"⟩;Code.part39;dropfelt ⟨"%19"⟩;dropfelt ⟨"%73"⟩;dropfelt ⟨"%77"⟩;dropfelt ⟨"%0"⟩;dropfelt ⟨"%81"⟩;dropfelt ⟨"%84"⟩;dropfelt ⟨"%88"⟩;dropfelt ⟨"%92"⟩;dropfelt ⟨"%96"⟩;dropfelt ⟨"%100"⟩;dropfelt ⟨"%104"⟩;dropfelt ⟨"%108"⟩;dropfelt ⟨"%112"⟩;dropfelt ⟨"%116"⟩;dropfelt ⟨"%120"⟩;dropfelt ⟨"%124"⟩;dropfelt ⟨"%128"⟩;dropfelt ⟨"%132"⟩;dropfelt ⟨"%136"⟩;dropfelt ⟨"%140"⟩;dropfelt ⟨"%144"⟩;dropfelt ⟨"%148"⟩;dropfelt ⟨"%152"⟩;dropfelt ⟨"%153"⟩;dropfelt ⟨"%155"⟩;dropfelt ⟨"%156"⟩;dropfelt ⟨"%157"⟩;dropfelt ⟨"%158"⟩;dropfelt ⟨"%159"⟩) st) ↔
+  Code.getReturn (MLIR.runProgram (Code.part14;dropfelt ⟨"%0"⟩;dropfelt ⟨"%56"⟩;dropfelt ⟨"%8"⟩;dropfelt ⟨"%57"⟩;dropfelt ⟨"%60"⟩;Code.part15;dropfelt ⟨"%61"⟩;dropfelt ⟨"%59"⟩;dropfelt ⟨"%62"⟩;dropfelt ⟨"%7"⟩;Code.part16;dropfelt ⟨"%6"⟩;dropfelt ⟨"%28"⟩;dropfelt ⟨"%43"⟩;dropfelt ⟨"%58"⟩;dropfelt ⟨"%63"⟩;dropfelt ⟨"%64"⟩) st) ↔
   Code.getReturn (part14_state_update st) := by
   unfold MLIR.runProgram; simp only
-  generalize eq : (dropfelt ⟨"%60"⟩;dropfelt ⟨"%14"⟩;dropfelt ⟨"%62"⟩;Code.part15;dropfelt ⟨"%63"⟩;dropfelt ⟨"%15"⟩;dropfelt ⟨"%65"⟩;Code.part16;dropfelt ⟨"%66"⟩;dropfelt ⟨"%16"⟩;dropfelt ⟨"%68"⟩;Code.part17;dropfelt ⟨"%69"⟩;dropfelt ⟨"%17"⟩;dropfelt ⟨"%71"⟩;Code.part18;dropfelt ⟨"%72"⟩;dropfelt ⟨"%18"⟩;dropfelt ⟨"%74"⟩;dropfelt ⟨"%75"⟩;dropfelt ⟨"%20"⟩;Code.part19;dropfelt ⟨"%76"⟩;Code.part20;dropfelt ⟨"%79"⟩;dropfelt ⟨"%80"⟩;dropfelt ⟨"%82"⟩;Code.part21;dropfelt ⟨"%21"⟩;dropfelt ⟨"%78"⟩;dropfelt ⟨"%83"⟩;dropfelt ⟨"%86"⟩;Code.part22;dropfelt ⟨"%22"⟩;dropfelt ⟨"%85"⟩;dropfelt ⟨"%87"⟩;dropfelt ⟨"%90"⟩;Code.part23;dropfelt ⟨"%25"⟩;dropfelt ⟨"%89"⟩;dropfelt ⟨"%91"⟩;dropfelt ⟨"%94"⟩;Code.part24;dropfelt ⟨"%28"⟩;dropfelt ⟨"%93"⟩;dropfelt ⟨"%95"⟩;dropfelt ⟨"%98"⟩;Code.part25;dropfelt ⟨"%31"⟩;dropfelt ⟨"%97"⟩;dropfelt ⟨"%99"⟩;dropfelt ⟨"%102"⟩;Code.part26;dropfelt ⟨"%34"⟩;dropfelt ⟨"%101"⟩;dropfelt ⟨"%103"⟩;dropfelt ⟨"%106"⟩;Code.part27;dropfelt ⟨"%37"⟩;dropfelt ⟨"%105"⟩;dropfelt ⟨"%107"⟩;dropfelt ⟨"%110"⟩;Code.part28;dropfelt ⟨"%40"⟩;dropfelt ⟨"%109"⟩;dropfelt ⟨"%111"⟩;dropfelt ⟨"%114"⟩;Code.part29;dropfelt ⟨"%43"⟩;dropfelt ⟨"%113"⟩;dropfelt ⟨"%115"⟩;dropfelt ⟨"%118"⟩;Code.part30;dropfelt ⟨"%46"⟩;dropfelt ⟨"%117"⟩;dropfelt ⟨"%119"⟩;dropfelt ⟨"%122"⟩;Code.part31;dropfelt ⟨"%49"⟩;dropfelt ⟨"%121"⟩;dropfelt ⟨"%123"⟩;dropfelt ⟨"%126"⟩;Code.part32;dropfelt ⟨"%52"⟩;dropfelt ⟨"%125"⟩;dropfelt ⟨"%127"⟩;dropfelt ⟨"%130"⟩;Code.part33;dropfelt ⟨"%55"⟩;dropfelt ⟨"%129"⟩;dropfelt ⟨"%131"⟩;dropfelt ⟨"%134"⟩;Code.part34;dropfelt ⟨"%58"⟩;dropfelt ⟨"%133"⟩;dropfelt ⟨"%135"⟩;dropfelt ⟨"%138"⟩;Code.part35;dropfelt ⟨"%61"⟩;dropfelt ⟨"%137"⟩;dropfelt ⟨"%139"⟩;dropfelt ⟨"%142"⟩;Code.part36;dropfelt ⟨"%64"⟩;dropfelt ⟨"%141"⟩;dropfelt ⟨"%143"⟩;dropfelt ⟨"%146"⟩;Code.part37;dropfelt ⟨"%67"⟩;dropfelt ⟨"%145"⟩;dropfelt ⟨"%147"⟩;dropfelt ⟨"%150"⟩;Code.part38;dropfelt ⟨"%70"⟩;dropfelt ⟨"%149"⟩;dropfelt ⟨"%151"⟩;dropfelt ⟨"%154"⟩;Code.part39;dropfelt ⟨"%19"⟩;dropfelt ⟨"%73"⟩;dropfelt ⟨"%77"⟩;dropfelt ⟨"%0"⟩;dropfelt ⟨"%81"⟩;dropfelt ⟨"%84"⟩;dropfelt ⟨"%88"⟩;dropfelt ⟨"%92"⟩;dropfelt ⟨"%96"⟩;dropfelt ⟨"%100"⟩;dropfelt ⟨"%104"⟩;dropfelt ⟨"%108"⟩;dropfelt ⟨"%112"⟩;dropfelt ⟨"%116"⟩;dropfelt ⟨"%120"⟩;dropfelt ⟨"%124"⟩;dropfelt ⟨"%128"⟩;dropfelt ⟨"%132"⟩;dropfelt ⟨"%136"⟩;dropfelt ⟨"%140"⟩;dropfelt ⟨"%144"⟩;dropfelt ⟨"%148"⟩;dropfelt ⟨"%152"⟩;dropfelt ⟨"%153"⟩;dropfelt ⟨"%155"⟩;dropfelt ⟨"%156"⟩;dropfelt ⟨"%157"⟩;dropfelt ⟨"%158"⟩;dropfelt ⟨"%159"⟩) = prog
+  generalize eq : (dropfelt ⟨"%0"⟩;dropfelt ⟨"%56"⟩;dropfelt ⟨"%8"⟩;dropfelt ⟨"%57"⟩;dropfelt ⟨"%60"⟩;Code.part15;dropfelt ⟨"%61"⟩;dropfelt ⟨"%59"⟩;dropfelt ⟨"%62"⟩;dropfelt ⟨"%7"⟩;Code.part16;dropfelt ⟨"%6"⟩;dropfelt ⟨"%28"⟩;dropfelt ⟨"%43"⟩;dropfelt ⟨"%58"⟩;dropfelt ⟨"%63"⟩;dropfelt ⟨"%64"⟩) = prog
   unfold Code.part14
   MLIR
   rewrite [←eq]
-  rewrite [MLIR.run_seq_def,MLIR.run_dropfelt, MLIR.run_seq_def,MLIR.run_dropfelt, MLIR.run_seq_def,MLIR.run_dropfelt]
+  rewrite [MLIR.run_seq_def,MLIR.run_dropfelt, MLIR.run_seq_def,MLIR.run_dropfelt, MLIR.run_seq_def,MLIR.run_dropfelt, MLIR.run_seq_def,MLIR.run_dropfelt, MLIR.run_seq_def,MLIR.run_dropfelt]
   unfold part14_state_update part14_drops part14_state
   rfl
 
@@ -44,56 +54,36 @@ lemma part14_updates_opaque {st : State} :
   Code.getReturn (part14_state_update (part13_drops (part13_state st))) := by
   simp [part13_state_update, part14_wp]
 
-lemma part14_cumulative_wp {x0 y0 y1 y2 y3 y4 y5 y6 y7 y8 y9 y10 y11 y12 y13 y14 y15 y16 y17 y18 y19: Felt} :
-  Code.run (start_state [x0] ([y0,y1,y2,y3,y4,y5,y6,y7,y8,y9,y10,y11,y12,y13,y14,y15,y16,y17,y18,y19])) ↔
+lemma part14_cumulative_wp {x0 x1 x2 x3 y0 y1 y2 y3 y4 y5 y6 y7 y8 y9 y10 y11 y12 y13 y14 y15 y16 y17: Felt} :
+  Code.run (start_state [x0,x1,x2,x3] ([y0,y1,y2,y3,y4,y5,y6,y7,y8,y9,y10,y11,y12,y13,y14,y15,y16,y17])) ↔
   Code.getReturn
       (part14_state_update
-        (((((((((((((((((({
-                                              buffers :=
-                                                ((fun x => Map.empty x)[{ name := "data" }] ←ₘ
-                                                    [[some y0, some y1, some y2, some y3, some y4, some y5, some y6,
-                                                        some y7, some y8, some y9, some y10, some y11, some y12,
-                                                        some y13, some y14, some y15, some y16, some y17, some y18,
-                                                        some y19]])[{ name := "code" }] ←ₘ
-                                                  [[some x0]],
-                                              bufferWidths :=
-                                                ((fun x => Map.empty x)[{ name := "data" }] ←ₘ
-                                                    20)[{ name := "code" }] ←ₘ
-                                                  1,
-                                              constraints := [], cycle := 0, felts := Map.empty, isFailed := false,
-                                              props := Map.empty,
-                                              vars :=
-                                                [{ name := "code" }, { name := "data" }] }[props][{ name := "%19" }] ←
-                                            True)[felts][{ name := "%22" }] ←
-                                          y2)[felts][{ name := "%21" }] ←
-                                        y1)[felts][{ name := "%25" }] ←
-                                      y3)[felts][{ name := "%28" }] ←
-                                    y4)[felts][{ name := "%31" }] ←
-                                  y5)[felts][{ name := "%34" }] ←
-                                y6)[felts][{ name := "%37" }] ←
-                              y7)[felts][{ name := "%40" }] ←
-                            y8)[felts][{ name := "%43" }] ←
-                          y9)[felts][{ name := "%46" }] ←
-                        y10)[felts][{ name := "%49" }] ←
-                      y11)[felts][{ name := "%52" }] ←
-                    y12)[felts][{ name := "%55" }] ←
-                  y13)[felts][{ name := "%58" }] ←
-                y14)[felts][{ name := "%60" }] ←
-              y1 + y2 * 2 + y3 * 3 + y4 * 4 + y5 * 5 + y6 * 6 + y7 * 7 + y8 * 8 + y9 * 9 + y10 * 10 + y11 * 11 +
-                    y12 * 12 +
-                  y13 * 13 +
-                y14 * 14)[felts][{ name := "%14" }] ←
-            15)[felts][{ name := "%61" }] ←
-          y15))  := by
+        (((((({
+                      buffers :=
+                        ((fun x => Map.empty x)[{ name := "data" }] ←ₘ
+                            [[some y0, some y1, some y2, some y3, some y4, some y5, some y6, some y7, some y8, some y9,
+                                some y10, some y11, some y12, some y13, some y14, some y15, some y16,
+                                some y17]])[{ name := "in" }] ←ₘ
+                          [[some x0, some x1, some x2, some x3]],
+                      bufferWidths := ((fun x => Map.empty x)[{ name := "data" }] ←ₘ 18)[{ name := "in" }] ←ₘ 4,
+                      constraints := [], cycle := 0, felts := Map.empty, isFailed := false, props := Map.empty,
+                      vars := [{ name := "in" }, { name := "data" }] }[props][{ name := "%6" }] ←
+                    True)[props][{ name := "%28" }] ←
+                  x3 - ((y10 * 64 + (y1 * 16 + y9 * 8 + y8 * 4 + y0)) * 2 + y13) = 0)[props][{ name := "%43" }] ←
+                (x3 - ((y10 * 64 + (y1 * 16 + y9 * 8 + y8 * 4 + y0)) * 2 + y13) = 0 ∧
+                  x2 - ((y12 * 8 + y2 * 2 + y11) * 16 + y4 * 4 + y3) = 0))[felts][{ name := "%0" }] ←
+              128)[felts][{ name := "%56" }] ←
+            y14 * 128 + (y15 * 4 + y5) * 16 + y7 * 4 + y6)[felts][{ name := "%8" }] ←
+          x1))  := by
     rewrite [part13_cumulative_wp]
     rewrite [part14_updates_opaque]
     unfold part13_state
-    MLIR_states_updates'
+    MLIR_states_updates
     -- 0 withEqZeros
     -- rewrite [withEqZero_def]
-    -- MLIR_states_updates'
+    -- MLIR_states_updates
     unfold part13_drops
-    -- 3 drops
+    -- 4 drops
     simp only [State.drop_update_swap, State.drop_update_same, State.drop_updateProps_swap]
     rewrite [State.dropFelts]
     simp only [State.dropFelts_buffers, State.dropFelts_bufferWidths, State.dropFelts_constraints, State.dropFelts_cycle, State.dropFelts_felts, State.dropFelts_isFailed, State.dropFelts_props, State.dropFelts_vars]
